orchestrating prover steps

pulse/lib/steel/pulse/Pulse.Prover.fst
@@ -1,5 +1,7 @@
 module Pulse.Prover
 
+open FStar.List.Tot
+
 open Pulse.Syntax
 open Pulse.Typing
 open Pulse.Checker.Common
@@ -7,9 +9,108 @@ open Pulse.Typing.Metatheory
 open Pulse.Checker.VPropEquiv
 open Pulse.Prover.Common
 
-module T = FStar.Tactics
+module ElimExists = Pulse.Prover.ElimExists
+module ElimPure =  Pulse.Prover.ElimPure
+module Match = Pulse.Prover.Match
+module IntroExists = Pulse.Prover.IntroExists
+
+module T = FStar.Tactics.V2
 
 module PS = Pulse.Prover.Substs
+
+let unsolved_equiv_pst (#preamble:_) (pst:prover_state preamble) (unsolved':list vprop)
+  (d:vprop_equiv (push_env pst.pg pst.uvs) (list_as_vprop pst.unsolved) (list_as_vprop unsolved'))
+  : prover_state preamble =
+  { pst with unsolved = unsolved'; goals_inv = magic () }
+
+let remaining_ctxt_equiv_pst (#preamble:_) (pst:prover_state preamble) (remaining_ctxt':list vprop)
+  (d:vprop_equiv pst.pg (list_as_vprop pst.remaining_ctxt) (list_as_vprop remaining_ctxt'))
+  : prover_state preamble =
+  { pst with remaining_ctxt = remaining_ctxt';
+             remaining_ctxt_frame_typing = magic ();
+             k = k_elab_equiv pst.k (VE_Refl _ _) (magic ()) }
+
+let rec collect_exists (g:env) (l:list vprop)
+  : exs:list vprop &
+    rest:list vprop &
+    vprop_equiv g (list_as_vprop l) (list_as_vprop (exs @ rest)) =
+  
+  match l with
+  | [] -> (| [], [], VE_Refl _ _ |)
+  | hd::tl ->
+    let (| exs, rest, _ |) = collect_exists g tl in
+    match hd.t with
+    | Tm_ExistsSL _ _ _ -> (| hd::exs, rest, magic () |)
+    | _ -> (| exs, hd::rest, magic () |)
+
+let rec collect_pures (g:env) (l:list vprop)
+  : pures:list vprop &
+    rest:list vprop &
+    vprop_equiv g (list_as_vprop l) (list_as_vprop (rest @ pures)) =
+  
+  match l with
+  | [] -> (| [], [], VE_Refl _ _ |)
+  | hd::tl ->
+    let (| pures, rest, _ |) = collect_pures g tl in
+    match hd.t with
+    | Tm_Pure _ -> (| hd::pures, rest, magic () |)
+    | _ -> (| pures, hd::rest, magic () |)
+
+
+module L = FStar.List.Tot
+let move_hd_end (g:env) (l:list vprop { Cons? l })
+  : vprop_equiv g (list_as_vprop l) (list_as_vprop (L.tl l @ [L.hd l])) = magic ()
+
+let rec match_q (#preamble:_) (pst:prover_state preamble)
+  (q:vprop) (unsolved':list vprop)
+  (_:squash (pst.unsolved == q::unsolved'))
+  (i:nat)
+  : T.Tac (option (pst':prover_state preamble { pst' `pst_extends` pst })) =
+
+  if L.length pst.remaining_ctxt = 0
+  then None
+  else if i = L.length pst.remaining_ctxt
+  then None
+  else
+    let p = L.hd pst.remaining_ctxt in
+    let pst_opt =
+      Match.match_step pst p (L.tl pst.remaining_ctxt) q unsolved' () in
+    match pst_opt with
+    | Some pst -> Some pst
+    | None ->
+      let pst =
+        remaining_ctxt_equiv_pst pst (L.tl pst.remaining_ctxt @ [L.hd pst.remaining_ctxt])
+          (move_hd_end pst.pg pst.remaining_ctxt) in
+      match_q pst q unsolved' () (i+1)
+
+let rec prover
+  (#preamble:_)
+  (pst0:prover_state preamble)
+  : T.Tac (pst':prover_state preamble { pst' `pst_extends` pst0 /\
+                                        is_terminal pst' }) =
+
+  match pst0.unsolved with
+  | [] -> pst0
+  | _ ->
+    let pst = ElimExists.elim_exists_pst pst0 in
+    let pst = ElimPure.elim_pure_pst pst in
+
+    let (| exs, rest, d |) = collect_exists (push_env pst.pg pst.uvs) pst.unsolved in
+    let pst = unsolved_equiv_pst pst (exs@rest) d in
+
+    match pst.unsolved with
+    | {t=Tm_ExistsSL u b body}::unsolved' ->
+      IntroExists.intro_exists pst u b body unsolved' () prover
+    | _ ->
+      let (| pures, rest, d |) = collect_pures (push_env pst.pg pst.uvs) pst.unsolved in
+      let pst = unsolved_equiv_pst pst (rest@pures) d in
+      match pst.unsolved with
+      | {t=Tm_Pure _}::tl -> fail pst.pg None "intro pure not implemented yet"  // only pures left
+      | q::tl ->
+        let pst_opt = match_q pst q tl () 0 in
+        match pst_opt with
+        | None -> fail pst.pg None "cannot match a vprop"
+        | Some pst -> prover pst  // a little wasteful?
 
 let prove
   (#g:env) (#ctxt:vprop) (ctxt_typing:vprop_typing g ctxt)
