pulse/lib/steel/pulse/Pulse.Prover.ElimExists.fsti
@@ -14,4 +14,5 @@ val elim_exists (#g:env) (#ctxt:term) (ctxt_typing:tot_typing g ctxt tm_vprop)
             continuation_elaborator g ctxt g' ctxt')
 
 val elim_exists_pst (#preamble:_) (pst:prover_state preamble)
-  : T.Tac (pst':prover_state preamble { pst' `pst_extends` pst })
+  : T.Tac (pst':prover_state preamble { pst' `pst_extends` pst /\
+                                        pst'.unsolved == pst.unsolved })
